examples/all_exists/CCR/wip.rl
@@ -1,3 +1,5 @@
+/* TODO linked list refinement. */
+
 interface List =
 
   class List
@@ -215,4 +217,4 @@ end
     }
 }
 
-
+ */
